theories/Example.v
@@ -1,22 +1,24 @@
 (**
 
-This file contains common declarations for examples in
-lifted Separation Logic, using lifted characteristic formulae.
+This file contains common declarations for examples in CFML 2.0.
 
 Author: Arthur Charguéraud.
 License: MIT.
 
 *)
 
-From Sep Require Export SepLifted LambdaCFLifted.
-From Sep Require Export LambdaStructLifted.
-From TLC Require Export LibList LibListZ.
+
+Set Implicit Arguments.
+Generalizable Variables A B.
+
+From Sep Require Export WPRecord.
+
+Export NotationForVariables NotationForTerms.
 Open Scope liblist_scope.
 Open Scope Z_scope.
-
-(* Open Scope charac. TODO: not needed? *)
-
-Ltac auto_star ::= jauto.
+Open Scope val_scope.
+Open Scope pat_scope.
+Open Scope trm_scope.
 
 
 (** Common preambule to be copied:
@@ -32,3 +34,20 @@ Implicit Types p : loc.
 Implicit Types n : int.
 
 *)
+
+(** Configuration of automation *)
+
+Ltac auto_false_base cont ::=
+  try solve [
+    intros_all; try match goal with |- _ <-> _ => split end;
+    solve [ cont tt
+          | intros_all; false;
+            solve [ try match goal with H: context [ _ <> _ ] |- _ => applys H; reflexivity end
+                  | cont tt ] ] ].
+
+Ltac auto_star ::=
+  try solve [ intuition eauto
+            | subst; rew_list in *; 
+              solve [ math 
+                    | auto_false_base ltac:(fun tt => intuition eauto) ] ].
+
