theories/ExamplePairing.v
@@ -1,0 +1,278 @@
+Set Implicit Arguments.
+Require Import FuncTactics LibCore.
+Require Import OrderedSig_ml HeapSig_ml OrderedSig_proof HeapSig_proof.
+Require Import PairingHeap_ml.
+
+Module PairingHeapSpec (O:MLOrdered) (OS:OrderedSigSpec with Module O:=O)
+  <: HeapSigSpec with Definition H.MLElement.t := O.t.
+
+(** instantiations *)
+
+Module Import H <: MLHeap := MLPairingHeap O.
+Module Import OS := OS.
+Existing Instance le_inst.
+Existing Instance le_order.
+
+(** invariant *)
+
+Definition is_ge (X Y:T) := X <= Y.
+
+Definition list_union (Hs:list (multiset T)) := 
+  fold_right union \{} Hs.
+
+Inductive inv : heap -> multiset T -> Prop :=
+  | inv_empty : 
+      inv Empty \{} 
+  | inv_node : forall x X hs Hs E,
+      rep x X ->
+      Forall2 inv hs Hs ->
+      Forall (fun H => H <> \{}) Hs ->
+      Forall (foreach (is_ge X)) Hs ->
+      E = \{X} \u list_union Hs ->   
+      inv (Node x hs) E.
+
+(** model *)
+
+Fixpoint size (t:heap) : nat :=
+  match t with
+  | Empty => 1%nat
+  | Node x hs => (1 + (1 + List.fold_right (fun t x => (x + size t)%nat) 0%nat hs)%nat)%nat 
+  end.
+
+Instance heap_rep : Rep heap (multiset T).
+Proof.
+  apply (Build_Rep inv). intros x. gen_eq n: (size x). gen x.
+  induction n using peano_induction; introv N HX HY; 
+  subst n; inverts HX; inverts HY; subst. prove_rep.
+  fequals. prove_rep. fequals. clear X X0 H0 H2 H3 H6 H8 H9. gen Hs Hs0.
+  induction hs; introv K1 K2; inverts K1; inverts K2. prove_rep. fequals.
+  applys* H. simpl; math. applys~ IHhs. intros. applys* H. simpls. math. 
+Defined.
+
+(** automation *)
+
+Hint Extern 1 (_ < _) => simpl; math.
+Hint Extern 1 (_ = _ :> multiset _) => permut_simpl : multiset.
+Hint Unfold removed_min.
+
+Definition U := multiset T.
+
+Ltac myauto cont :=
+  match goal with 
+  | |- _ = _ :> LibSet.set ?T => try solve [ change (multiset T) with U; cont tt ]
+  | |- _ => cont tt
+  end.
+
+Ltac auto_tilde ::= myauto ltac:(fun _ => eauto).
+Ltac auto_star ::= try solve [ intuition (eauto with multiset) ].
+
+Hint Constructors inv Forall Forall2.
+
+(** useful facts *)
+
+Lemma foreach_ge_trans : forall (X Y : OS.T) (E : multiset OS.T),
+  foreach (is_ge X) E -> Y <= X -> foreach (is_ge Y) E.
+Proof. intros. apply~ foreach_weaken. intros_all. apply* le_trans. Qed.
+
+Hint Resolve foreach_ge_trans.
+
+Lemma min_of_prove : forall (X : OS.T) (Hs : list (multiset OS.T)),
+  Forall (foreach (is_ge X)) Hs ->
+  min_of ('{X} \u list_union Hs) X.
+Proof.
+  introv H. split~. introv M. destruct (in_union_inv M) as [N|N].
+  rewrite (in_single N). apply le_refl.
+  clear M. unfolds list_union. induction Hs; simpls.
+    false. eapply in_empty. eauto.
+    inversions H. destruct (in_union_inv N) as [P|P].
+      apply~ H3.
+      apply~ IHHs.
+Qed.
+
+Hint Resolve min_of_prove.
+
+(** verification *)
+
+Lemma empty_spec : rep empty \{}.
+Proof. apply empty_cf. xret~. Qed.
+
+Hint Extern 1 (RegisterSpec empty) => Provide empty_spec.
+
+Lemma is_empty_spec : RepTotal is_empty (E;heap) >> 
+  bool_of (E = \{}).
+Proof.
+  xcf. intros e E RepE. inverts RepE; xgo. 
+  auto. multiset_inv.
+Qed. 
+
+Hint Extern 1 (RegisterSpec is_empty) => Provide is_empty_spec.
+
+Lemma merge_spec : RepTotal merge (E1;heap) (E2;heap) >>
+  E1 \u E2 ;- heap.
+Proof.
+  xcf. introv Rep1 Rep2. xmatch.
+  xgo. inverts Rep2. equates* 1.
+  xgo. inverts Rep1. equates* 1.
+  xcleanpat. inverts keep Rep1. inverts keep Rep2. xgo~.
+    constructors.
+      eauto.
+      eauto. 
+      constructors~. multiset_inv.
+      clear H6 H7 Rep2. constructors. eauto. rew_foreach. splits~.
+       applys (@foreach_weaken _ (is_ge X0)).
+         unfold list_union. induction Hs0; simpl. auto. inverts~ H8.
+         intros_all. applys~ le_trans.
+    unfold list_union. simple*.
+    lets: (nle_to_sle P_x0). constructors.
+      eauto.
+      eauto. 
+      constructors~. multiset_inv.
+      clear H2 H3 Rep1. constructors. eauto. rew_foreach. splits~.
+       applys (@foreach_weaken _ (is_ge X)).
+         unfold list_union. induction Hs; simpl. auto. inverts~ H4.
+         intros_all. applys~ le_trans.
+    unfold list_union. simpl. permut_simpl.
+Qed.
+
+Hint Extern 1 (RegisterSpec merge) => Provide merge_spec.
+
+Lemma insert_spec : RepTotal insert (X;O.t) (E;heap) >>
+  \{X} \u E ;- heap.
+Proof.
+  xcf. introv RepX RepE. xapp~ (>>> \{X} E).
+  applys~ (>>> inv_node X (@nil (multiset T))).
+  unfolds list_union. simple*.
+Qed.
+
+Hint Extern 1 (RegisterSpec insert) => Provide insert_spec.
+
+Lemma merge_pairs_spec : Spec merge_pairs hs |R>>
+  forall Hs, 
+  Forall2 inv hs Hs ->
+  Forall (fun H => H <> \{}) Hs -> 
+  R (list_union Hs ;- heap).
+Proof.
+  xinduction (@List.length heap). xcf. introv IH RepH NE. xmatch.
+  xgo. inverts~ RepH.
+  xgo. inverts RepH. inverts H2. unfolds list_union. simpls. equates* 1.
+  xcleanpat. inverts RepH. inverts H2. inverts NE. inverts H2.
+   xgo~. ximpl. equates* 1.
+Qed.
+
+Hint Extern 1 (RegisterSpec merge_pairs) => Provide merge_pairs_spec.
+
+Lemma find_min_spec : RepSpec find_min (E;heap) |R>>
+  E <> \{} -> R (min_of E ;; O.t).
+Proof.
+  xcf. intros e E RepE HasE. inverts RepE; xgo*.
+Qed.
+
+Hint Extern 1 (RegisterSpec find_min) => Provide find_min_spec.
+
+Lemma delete_min_spec : RepSpec delete_min (E;heap) |R>>
+  E <> \{} -> R (removed_min E ;; heap).
+Proof. 
+  xcf. intros e E RepE HasE. inverts RepE; xgo~. ximpl. xrep~.
+Qed.
+
+Hint Extern 1 (RegisterSpec delete_min) => Provide delete_min_spec.
+
+End PairingHeapSpec.
+
+
+
+
+
+
+(* https://sites.google.com/site/progyumming/cpp/pairing-heap
+
+https://github.com/saadtaame/pairing-heap/blob/master/pairing_heap.cc
+
+https://www.sanfoundry.com/cpp-program-implement-pairing-heap/
+
+https://www.techiedelight.com/deletion-from-bst/
+
+
+module PairingHeap (Element : Ordered) : Heap =
+  (* (Heap with module Element = Element)*)
+struct
+  module Element = Element
+
+
+  type heap = Empty | Node of Element.t * heap list
+
+  let empty = Empty
+
+  let is_empty = function
+     | Empty -> true
+     | _ -> false
+
+  let merge h1 h2 = 
+     match h1, h2 with
+     | _, Empty -> h1
+     | Empty, _ -> h2
+     | Node (x, hs1), Node (y, hs2) ->
+         if Element.leq x y 
+            then Node (x, h2 :: hs1)
+            else Node (y, h1 :: hs2)
+
+  let insert x h = 
+     merge (Node (x, [])) h
+
+  let rec merge_pairs = function
+     | [] -> Empty
+     | [h] -> h
+     | h1::h2::hs -> merge (merge h1 h2) (merge_pairs hs)
+
+  let find_min = function 
+     | Empty -> raise EmptyStructure 
+     | Node (x, _) -> x
+
+  let delete_min = function 
+     | Empty -> raise EmptyStructure 
+     | Node (x, hs) -> merge_pairs hs
+
+end
+
+
+
+type pairing_heap = ref node
+
+  create() =
+    ref null
+
+	let is_empty p =
+		return (!p == null)
+
+	let pop_front p =
+		if (empty p) fail
+    int x = !p.value;
+    root = merge_pairs(!p->sub);
+		return x
+
+type node = { 
+		int value;
+		node* parent;
+		mlist<node*> sub;
+};
+
+let merge(node * a, node * b)  : node* =
+		if (a == null) return b;
+		if (b == null) return a;
+		if (!a.value < !b.value) {
+			!a.sub.push_front(b);
+			return a;
+		} else {
+			!b.sub.push_front(a);
+			return b;
+		}
+	}
+	node * merge_pairs(list<node*> s) {
+    if s.is_empty() return null else
+    let a = s.pop_front()
+    if s.is_empty() return a else
+    let b = s.pop_front()
+		return merge(merge(a, b), merge_pairs(s));
+	}
+
+*)
