theories/ExampleStack.v
@@ -1,0 +1,286 @@
+(**
+
+This file provides examples of the verification of a stack,
+using CFML 2.0.
+
+Author: Arthur Charguéraud.
+License: MIT.
+
+*)
+
+
+Set Implicit Arguments.
+Generalizable Variables A B.
+From Sep Require Import Example.
+
+
+
+(* ********************************************************************** *)
+(* * Stack *)
+
+(** Implementation of a stack as a reference on a list *)
+
+Module Stack.
+
+(** OCaml syntax
+[[
+
+  type 'a stack = ('a list) ref
+
+  let create () =
+    ref []
+
+  let is_empty p =
+    !p = []
+
+  let push p x =
+    p := x :: !p
+
+  let pop p =
+    match !p with
+    | [] -> raise Not_found
+    | x::r -> p := r; x
+
+  let rev_append f p1 p2 =
+    if not (is_empty p1) then begin
+      let x = pop p1 in
+      push p2 x;
+      f p1 p2
+    end
+]]
+*)
+
+(** Code *)
+
+Definition create : val :=
+  VFun 'u :=
+   val_ref 'nil.
+
+Definition is_empty : val :=
+  VFun 'p :=
+    val_get 'p '= 'nil.
+
+Definition push : val :=
+  VFun 'p 'x :=
+   'p ':= ('x ':: (val_get 'p)).
+
+Definition pop : val :=
+  VFun 'p :=
+   Let 'q := val_get 'p in
+   Match 'q With
+   '| 'nil '=> 'Fail
+   '| 'x ':: 'r '=> ('p ':= 'r) '; 'x
+   End.
+
+Definition rev_append : val :=
+  VFix 'f 'p1 'p2 :=
+    If_ 'not (is_empty 'p1) Then
+       Let 'x := pop 'p1 in
+       push 'p2 'x ';
+       'f 'p1 'p2
+    End.
+
+(** Representation predicate *)
+
+Definition Stack `{Enc A} (L:list A) (p:loc) : hprop :=
+  p ~~> L.
+
+(** Verification *)
+
+Lemma Triple_create : forall `{Enc A} (u:unit),
+  TRIPLE (create u)
+    PRE \[]
+    POST (fun p => (p ~> Stack (@nil A))).
+Proof using.
+  xwp. xval nil. xapp. hsimpl.
+Qed.
+
+Hint Extern 1 (Register_Spec create) => Provide @Triple_create.
+
+Lemma Triple_is_empty : forall `{Enc A} (p:loc) (L:list A),
+  TRIPLE (is_empty p)
+    PRE (p ~> Stack L)
+    POST (fun (b:bool) => \[b = isTrue (L = nil)] \* p ~> Stack L).
+Proof using.
+  xwp. xunfold Stack. xapp. xval nil.
+  xapp~ @Triple_eq_r. hsimpl*.
+Qed.
+
+Hint Extern 1 (Register_Spec is_empty) => Provide @Triple_is_empty.
+
+Lemma Triple_push : forall `{Enc A} (p:loc) (x:A) (L:list A),
+  TRIPLE (push p (``x))
+    PRE (p ~> Stack L)
+    POST (fun (u:unit) => (p ~> Stack (x::L))).
+Proof using.
+  xwp. xunfold Stack. xapp. xval (x::L). xapp. hsimpl.
+Qed.
+
+Hint Extern 1 (Register_Spec push) => Provide @Triple_push.
+
+Lemma Triple_pop : forall `{Enc A} (p:loc) (L:list A),
+  L <> nil ->
+  TRIPLE (pop p)
+    PRE (p ~> Stack L)
+    POST (fun (x:A) => \exists L', \[L = x::L'] \* (p ~> Stack L')).
+Proof using.
+  introv N. xwp. xunfold Stack. xapp.
+  applys xmatch_lemma_list.
+  { intros HL. xfail. }
+  { intros X L' HL. xapp. xval. hsimpl~. }
+Qed.
+
+Hint Extern 1 (Register_Spec pop) => Provide @Triple_pop.
+
+Opaque Stack.
+
+Lemma Triple_rev_append : forall `{Enc A} (p1 p2:loc) (L1 L2:list A),
+  TRIPLE (rev_append p1 p2)
+    PRE (p1 ~> Stack L1 \* p2 ~> Stack L2)
+    POST (fun (u:unit) => p1 ~> Stack nil \* p2 ~> Stack (rev L1 ++ L2)).
+Proof using.
+  intros. gen p1 p2 L2. induction_wf IH: (@list_sub A) L1. intros.
+  xwp. xapp. xapp. xif ;=> C.
+  { (* case cons *)
+    xapp~ ;=> x L1' E. xapp. xapp. { subst*. } hsimpl. subst. rew_list~. }
+  { (* case nil *)
+    xval tt. hsimpl~. subst. rew_list~. }
+Qed.
+
+Hint Extern 1 (Register_Spec rev_append) => Provide @Triple_rev_append.
+
+End Stack.
+
+
+
+(* ********************************************************************** *)
+(* * Stack with length *)
+
+(** Implementation of a stack with a size as a record made of
+    a list and a size field *)
+
+Module Stackn.
+
+(** OCaml syntax
+[[
+  type 'a lstack = { data : 'a list; size : int }
+
+  let create () =
+    { data = []; size = 0 }
+
+  let is_empty p =
+    p.size = 0
+
+  let push p x =
+    p.data <- x :: p.data;
+    p.size <- p.size + 1
+
+  let pop p =
+    match !p.data with
+    | [] -> raise Not_found
+    | x::r -> 
+        p.data <- r;
+        p.size <- p.size - 1;
+        x
+
+   let clear p =  
+     p.data <- [];
+     p.size <- 0
+
+   let concat p1 p2 =
+     p1.data <- p1.data @ p2.data;
+     p1.size <- p1.size + p2.size;
+     clear p2
+]]
+*)
+
+(** Source code *)
+
+Definition data : field := 0%nat.
+Definition size : field := 1%nat.
+
+Definition is_empty : val :=
+  VFun 'p :=
+    'p'.size '= 0.
+
+Definition val_push : val :=
+  VFun 'p 'x :=
+   Set 'p'.data ':= ('x ':: 'p'.data) ';
+   Set 'p'.size ':= ('p'.size '+ 1).
+
+Definition val_pop : val :=
+  VFun 'p :=
+   Let 'q := 'p'.data in 
+   Match 'q With (* LATER: allow inline *)
+   '| 'nil '=> 'Fail
+   '| 'x ':: 'r '=> 
+       Set 'p'.data ':= 'r ';
+       Set 'p'.size ':= ('p'.size '- 1) ';
+       'x
+   End.
+
+(** Representation predicate *)
+
+Definition Stackn `{Enc A} (L:list A) (p:loc) : hprop :=
+  p ~> Record`{ data := L; size := LibListZ.length L }.
+
+
+(** Verification *)
+
+Lemma Triple_is_empty : forall `{Enc A} (p:loc) (L:list A),
+  TRIPLE (is_empty p)
+    PRE (p ~> Stackn L)
+    POST (fun (b:bool) => \[b = isTrue (L = nil)] \* p ~> Stackn L).
+Proof using.
+  xwp. xunfold Stackn. xapp. xapp~. hsimpl.
+  rewrite* LibListZ_length_zero_eq_eq_nil.
+Qed.
+
+Lemma Triple_push : forall `{Enc A} (p:loc) (x:A) (L:list A),
+  TRIPLE (val_push p (``x))
+    PRE (p ~> Stackn L)
+    POST (fun (u:unit) => (p ~> Stackn (x::L))).
+Proof using.
+  xwp. xunfold Stackn. xapp. xval (x::L). xappn.
+  hsimpl. (* LATER: hsimpl could do xrecord_eq *) 
+  xrecord_eq. rew_list; math.
+Qed.
+
+Lemma Triple_pop : forall `{Enc A} (p:loc) (L:list A),
+  L <> nil ->
+  TRIPLE (val_pop p)
+    PRE (p ~> Stackn L)
+    POST (fun (x:A) => \exists L', \[L = x::L'] \* (p ~> Stackn L')).
+Proof using.
+  introv N. xwp. xunfold Stackn. xapp.
+  applys xmatch_lemma_list.
+  { intros HL. xfail. }
+  { intros X L' HL. xappn. xval. hsimpl*. 
+    (* LATER:  hsimpl could do xrecord_eq *) 
+    xrecord_eq. subst; rew_list; math. }
+Qed.
+
+Opaque Stackn.
+
+
+(*
+Lemma Triple_get_field : forall (l:loc) f `{EA:Enc A} (V:A),
+  TRIPLE ((val_get_field f) l)
+    PRE (l `.` f ~~> V)
+    POST (fun r => \[r = V] \* (l `.` f ~~> V)).
+Proof using.
+*)
+
+(*
+Lemma Triple_create : forall `{Enc A} (u:unit),
+  TRIPLE (val_create u)
+    PRE \[]
+    POST (fun p => (p ~> Stackn (@nil A))).
+Proof using.
+  xwp. xval nil. xapp~.
+Qed.
+*)
+
+
+
+End Stackn.
